src/spec/Flutterbye.Seq.Mem.fst
@@ -1,30 +1,30 @@
 // $legal:635:
-// 
+//
 // Copyright 2016 Michael Lowell Roberts & Microsoft Research
-// 
+//
 // Licensed under the Apache License, Version 2.0 (the "License");
 // you may not use this file except in compliance with the License.
 // You may obtain a copy of the License at
-// 
+//
 //     http://www.apache.org/licenses/LICENSE-2.0
-// 
+//
 // Unless required by applicable law or agreed to in writing, software
 // distributed under the License is distributed on an "AS IS" BASIS,
 // WITHOUT WARRANTIES OR CONDITIONS OF ANY KIND, either express or implied.
 // See the License for the specific language governing permissions and
 // limitations under the License.
-// 
+//
 // ,$
 
 module Flutterbye.Seq.Mem
 open FStar.Seq
 open Flutterbye.Seq.Find
 
-type Mem (#a:Type) (x:a) (s:seq a) =
+type mem_t (#a:Type) (x:a) (s:seq a) =
    exists (i:nat).
       i < length s && index s i = x
 
-val mem: x:'a -> s:seq 'a -> Tot (b:bool{b <==> Mem x s})
+val mem: x:'a -> s:seq 'a -> Tot (b:bool{b <==> mem_t x s})
 let mem a s =
    is_Some (find a s)
 
@@ -33,7 +33,7 @@ val lemma__index:
    -> i:nat{i < length s}
    -> Lemma
       (requires (True))
-      (ensures (mem (index s i) s))
+      (ensures (mem_t (index s i) s))
 let lemma__index s i =
    lemma__find (index s i) s
 
@@ -41,11 +41,11 @@ val lemma__slice_1:
    a:'a
    -> s:seq 'a
    -> Lemma
-      (requires (mem a s))
+      (requires (mem_t a s))
       (ensures
          (forall (i:nat) (j:nat) (q:seq 'a).
-            ((j < length q /\ i <= j /\ (Eq s (slice q i j))) ==>
-               mem a q)))
+            ((j < length q /\ i <= j /\ (equal s (slice q i j))) ==>
+               mem_t a q)))
 let lemma__slice_1 a s =
    ()
 
@@ -55,11 +55,11 @@ val lemma__slice_2:
    a:'a
    -> s:seq 'a
    -> Lemma
-      (requires (mem a s))
+      (requires (mem_t a s))
       (ensures
          (forall (i:nat).
             ((i < length s && index s i = a) ==>
-               (mem a (slice s 0 (i + 1))))))
+               (mem_t a (slice s 0 (i + 1))))))
 let lemma__slice_2 a s =
    ()
 
@@ -68,8 +68,8 @@ private val lemma__append__case_1:
    -> s_1:seq 'a
    -> s_2:seq 'a
    -> Lemma
-      (requires (mem x s_1))
-      (ensures (mem x (append s_1 s_2)))
+      (requires (mem_t x s_1))
+      (ensures (mem_t x (append s_1 s_2)))
 let lemma__append__case_1 x s_1 s_2 =
    ()
 
@@ -78,8 +78,8 @@ private val lemma__append__case_2:
    -> s_1:seq 'a
    -> s_2:seq 'a
    -> Lemma
-      (requires (mem x s_2))
-      (ensures (mem x (append s_1 s_2)))
+      (requires (mem_t x s_2))
+      (ensures (mem_t x (append s_1 s_2)))
 let lemma__append__case_2 x s_1 s_2 =
    let s' = append s_1 s_2 in
    let i = length s_1 in
@@ -93,8 +93,8 @@ val lemma__append:
    -> s_1:seq 'a
    -> s_2:seq 'a
    -> Lemma
-      (requires (mem x s_1 || mem x s_2))
-      (ensures (mem x (append s_1 s_2)))
+      (requires (mem_t x s_1 \/ mem_t x s_2))
+      (ensures (mem_t x (append s_1 s_2)))
 let lemma__append x s_1 s_2 =
    if mem x s_1 then
       lemma__append__case_1 x s_1 s_2
@@ -106,7 +106,7 @@ val lemma__empty:
    -> s:seq 'a
    -> Lemma
       (requires (length s = 0))
-      (ensures (not (mem x s)))
+      (ensures (~ (mem_t x s)))
       [SMTPat (mem x s)]
 let lemma__empty x s = ()
 
@@ -115,6 +115,9 @@ val lemma__create:
    -> a:'a
    -> Lemma
       (requires (True))
-      (ensures (mem a (create n a)))
+      (ensures (mem_t a (create n a)))
       [SMTPat (create n a)]
-let lemma__create n a = ()
+let lemma__create n a =
+   let s = create n a in
+   assert (index s 0 = a);
+   ()
